@prefix : <http://romanrepublic.ac.uk/rdf/ontology#> .
@prefix owl: <http://www.w3.org/2002/07/owl#> .
@prefix rdf: <http://www.w3.org/1999/02/22-rdf-syntax-ns#> .
@prefix xml: <http://www.w3.org/XML/1998/namespace> .
@prefix xsd: <http://www.w3.org/2001/XMLSchema#> .
@prefix rdfs: <http://www.w3.org/2000/01/rdf-schema#> .

<http://romanrepublic.ac.uk/rdf/ontology#> a owl:Ontology ;
	owl:versionInfo "1.0"^^xsd:decimal ;
	rdfs:comment "An ontology for the data created by the Digital Prosopography of the Roman Republic project (see http://www.romanrepublic.ac.uk).  The major data repository for the work of the DPRR project was a relational database.  This ontology provides a definition of an RDF expression of the data in that database." ;
	rdfs:label "Ontology for DPRR data" .
# 
# 
# #################################################################
# #
# #    Annotation properties
# #
# #################################################################
# 
# 
# http://romanrepublic.ac.uk/rdf/ontology#hasPersonName

:hasPersonName a owl:AnnotationProperty ;
	rdfs:subPropertyOf rdfs:label ;
	rdfs:range xsd:string ;
	rdfs:domain :Person .
# 
# 
# 
# #################################################################
# #
# #    Object Properties
# #
# #################################################################
# 
# 
# http://romanrepublic.ac.uk/rdf/ontology#forAssertion

:forAssertion a owl:ObjectProperty ;
	rdfs:domain :PrimarySourceReference ;
	rdfs:range :Assertion .
# 
# http://romanrepublic.ac.uk/rdf/ontology#forRelationship

:forRelationship a owl:ObjectProperty ;
	rdfs:domain :RelationshipInverse ;
	rdfs:range :Relationship ;
	rdfs:comment "use this property (one of two, see also :forSex) to lookup the inverse of a given relationship" ;
	rdfs:seeAlso "The other \"lookup\" property is :forSex" .
# 
# http://romanrepublic.ac.uk/rdf/ontology#forSex

:forSex a owl:ObjectProperty ;
	rdfs:domain :RelationshipInverse ;
	rdfs:range :Sex ;
	rdfs:comment "use this property with :forRelationship to look up the inverse of a given relationship" ;
	rdfs:seeAlso "to use :RelationshipInverse as a lookup mechanism, one must also provide :forRelationship" .
# 
# http://romanrepublic.ac.uk/rdf/ontology#hasAltPraenomen

:hasAltPraenomen a owl:ObjectProperty ;
	rdfs:domain :Person ;
	rdfs:range :Praenomen ;
	rdfs:comment "provides what DPRR considers to be an alternative Praenomen for the person." .
# 
# http://romanrepublic.ac.uk/rdf/ontology#hasAssertedRelationshipInverse

:hasAssertedRelationshipInverse a owl:ObjectProperty ;
	rdfs:domain :RelationshipAssertion ;
	rdfs:range :RelationshipAssertion .
# 
# http://romanrepublic.ac.uk/rdf/ontology#hasDateSecondarySource

:hasDateSecondarySource a owl:ObjectProperty ;
	rdfs:domain :AssertionWithDateRange ;
	rdfs:range :SecondarySource ;
	rdfs:comment "A link to a secondary source that supports the dates given in this assertion." .
# 
# http://romanrepublic.ac.uk/rdf/ontology#hasDateType

:hasDateType a owl:ObjectProperty ;
	rdfs:domain :DateInformation ;
	rdfs:range :DateType ;
	rdfs:comment "The kind of life event (e,g, attestation, birth or death date, date of exile, etc) that this instance is referring to." .
# 
# http://romanrepublic.ac.uk/rdf/ontology#hasInverseRelationship

:hasInverseRelationship a owl:ObjectProperty ;
	rdfs:domain :RelationshipInverse ;
	rdfs:range :Relationship ;
	rdfs:comment "A mechanism to allow DPRR to assert the particular inverse relationship that applies for the particular relationship being specified. For example, if A is father of B there are two possible inverse relationships: B is son of A or B is daughter of A.  This mechanism allows DPRR to make explicit which one applies." .
# 
# http://romanrepublic.ac.uk/rdf/ontology#hasNoteType

:hasNoteType a owl:ObjectProperty ;
	rdfs:domain :Note ;
	rdfs:range :NoteType ;
	rdfs:comment "In some sources (Broughton and Ruepke in particular) notes provided are typed.  This is the place where the type of note (for these and other sources) is specified." .
# 
# http://romanrepublic.ac.uk/rdf/ontology#hasOffice

:hasOffice a owl:ObjectProperty ;
	rdfs:domain :PostAssertion ;
	rdfs:range :Office ;
	rdfs:comment "links to the :Office that is attached to the post in this assertion." .
# 
# http://romanrepublic.ac.uk/rdf/ontology#hasParent

:hasParent a owl:ObjectProperty ;
	rdfs:domain :HierarchicalAuthority ;
	rdfs:range :HierarchicalAuthority ;
	rdfs:comment "used in authority lists that have a hierarchical structure to provide the hierarchical parent for each instance." .
# 
# http://romanrepublic.ac.uk/rdf/ontology#hasPersonNote

:hasPersonNote a owl:ObjectProperty ;
	rdfs:domain :Person ;
	rdfs:range :PersonNote ;
	rdfs:comment "links to one or more notes about the person that DPRR has recorded as :PersonNote instances." .
# 
# http://romanrepublic.ac.uk/rdf/ontology#hasPostAssertion

:hasPostAssertion a owl:ObjectProperty ;
	rdfs:domain :PostAssertionProvince ;
	rdfs:range :PostAssertion ;
	rdfs:comment "A :PostAssertionProvince class is mean to link a :PostAssertion to a :Province.  This is the pointer to the :PostAssertion" .
# 
# http://romanrepublic.ac.uk/rdf/ontology#hasPostAssertionNote

:hasPostAssertionNote a owl:ObjectProperty ;
	rdfs:domain :PostAssertion ;
	rdfs:range :PostAssertionNote ;
	rdfs:comment "A link to a :PostAssertionNote that is connected to this :PostAssertion" .
# 
# http://romanrepublic.ac.uk/rdf/ontology#hasPraenomen

:hasPraenomen a owl:ObjectProperty ;
	rdfs:domain :Person ;
	rdfs:range :Praenomen ;
	rdfs:comment "links to the primary Praenomen associated with this person." ;
	rdfs:seeAlso ":hasAltPraenomen" .
# 
# http://romanrepublic.ac.uk/rdf/ontology#hasPrimarySource

:hasPrimarySource a owl:ObjectProperty ;
	rdfs:domain :PrimarySourceReference ;
	rdfs:range :PrimarySource ;
	rdfs:comment "links this :PrimarySourceReference to a :PrimarySource" .
# 
# http://romanrepublic.ac.uk/rdf/ontology#hasProvince

:hasProvince a owl:ObjectProperty ;
	rdfs:domain :NoteForProvince ;
	rdfs:range :Province ;
	rdfs:comment ":PostAssertionProvince and :StatusAssertionProvince classes are mean to link a :PostAssertion or :StatusAssertion to a :Province.  This is the pointer to the :Province in it." .
# 
# http://romanrepublic.ac.uk/rdf/ontology#hasRelatedPerson

:hasRelatedPerson a owl:ObjectProperty ;
	rdfs:domain :RelationshipAssertion ;
	rdfs:range :Person ;
	rdfs:comment "provides the reference to the 2nd person in a relationship.  If A is mother of B, then :hasRelatedPerson will point to B." ;
	rdfs:seeAlso "If A is mother of B, the person pointer shared by all assertions (:hasPerson) will point to A." .
# 
# http://romanrepublic.ac.uk/rdf/ontology#hasRelatedRelationship

:hasRelatedRelationship a owl:ObjectProperty ;
	rdfs:domain :RelationshipAssertion ;
	rdfs:range :RelationshipAssertion ;
	rdfs:comment "allows two relationship assertions that are related in DPRR's view to be connected." .
# 
# http://romanrepublic.ac.uk/rdf/ontology#hasRelationship

:hasRelationship a owl:ObjectProperty ;
	rdfs:domain :RelationshipAssertion ;
	rdfs:range :Relationship ;
	rdfs:comment "points to the particular :Relationship that this relationahip assertion is making." .
# 
# http://romanrepublic.ac.uk/rdf/ontology#hasRelationshipReference

:hasRelationshipReference a owl:ObjectProperty ;
	rdfs:domain :RelationshipAssertion ;
	rdfs:range :RelationshipAssertionReference .
# 
# http://romanrepublic.ac.uk/rdf/ontology#hasSecondarySource

:hasSecondarySource a owl:ObjectProperty ;
	rdfs:domain :Assertion ;
	rdfs:range :SecondarySource ;
	rdfs:comment "Specifies the original secondary source that DPRR used for the information." .
# 
# http://romanrepublic.ac.uk/rdf/ontology#hasSecondarySourceForNote

:hasSecondarySourceForNote a owl:ObjectProperty ;
	rdfs:domain :Note ;
	rdfs:range :SecondarySource ;
	rdfs:comment "Specifies the original secondary source that DPRR used for the information in this Note." .
# 
# http://romanrepublic.ac.uk/rdf/ontology#hasStatus

:hasStatus a owl:ObjectProperty ;
	rdfs:domain :StatusAssertion ;
	rdfs:range :Status ;
	rdfs:comment "links a status assertion to the particular status that applies" .
# 
# http://romanrepublic.ac.uk/rdf/ontology#hasStatusAssertion

:hasStatusAssertion a owl:ObjectProperty ;
	rdfs:domain :StatusAssertionProvince ;
	rdfs:range :StatusAssertion ;
	rdfs:comment "connects a :Province to a :StatusAssertion" .
# 
# http://romanrepublic.ac.uk/rdf/ontology#hasStatusAssertionNote

:hasStatusAssertionNote a owl:ObjectProperty ;
	rdfs:domain :StatusAssertion ;
	rdfs:range :StatusAssertionNote ;
	rdfs:comment "links the assertion to the particular note (:StatusAssertionNote) that applies" .
# 
# http://romanrepublic.ac.uk/rdf/ontology#hasTribe

:hasTribe a owl:ObjectProperty ;
	rdfs:domain :TribeAssertion ;
	rdfs:range :Tribe ;
	rdfs:comment "in :TribeAssertion specifies which :Tribe is being asserted." .
# 
# http://romanrepublic.ac.uk/rdf/ontology#isAboutPerson

:isAboutPerson a owl:ObjectProperty ;
	rdfs:domain :Assertion ;
	rdfs:range :Person ;
	rdfs:comment "Connects the assertion to the person the assertion is about." .
# 
# http://romanrepublic.ac.uk/rdf/ontology#isSex

:isSex a owl:ObjectProperty ;
	rdfs:domain :Person ;
	rdfs:range :Sex ;
	rdfs:comment "the Sex of the person." .
# 
# 
# 
# #################################################################
# #
# #    Data properties
# #
# #################################################################
# 
# 
# http://romanrepublic.ac.uk/rdf/ontology#hasAbbreviation

:hasAbbreviation a owl:DatatypeProperty ;
	rdfs:domain :AuthorityWithAbbreviation ;
	rdfs:range xsd:string ;
	rdfs:comment "Provides a text string that is the abbreviated form of the name for the authority list item" .
# 
# http://romanrepublic.ac.uk/rdf/ontology#hasBiblio

:hasBiblio a owl:DatatypeProperty ;
	rdfs:domain :Source ;
	rdfs:range xsd:string ;
	rdfs:comment "A bilbiographic reference for the source." .
# 
# http://romanrepublic.ac.uk/rdf/ontology#hasCognomen

:hasCognomen a owl:DatatypeProperty ;
	rdfs:domain :Person ;
	rdfs:range xsd:string ;
	rdfs:comment "A text string for the person's Cognomen" .
# 
# http://romanrepublic.ac.uk/rdf/ontology#hasDateDisplayText

:hasDateDisplayText a owl:DatatypeProperty ;
	rdfs:domain :AssertionWithDateRange ;
	rdfs:range xsd:string ;
	rdfs:comment "A field to contain a comment about the range of dates when DPRR believed a status or post applied.  Rarely used." ;
	rdfs:seeAlso "See :hasDisplaySourceText" .
# 
# http://romanrepublic.ac.uk/rdf/ontology#hasDateEnd

:hasDateEnd a owl:DatatypeProperty ;
	rdfs:domain :AssertionWithDateRange ;
	rdfs:range xsd:integer ;
	rdfs:comment "provides a date (a year) which is the endpoint for the period of time covered by the assertion." .
# 
# http://romanrepublic.ac.uk/rdf/ontology#hasDateInterval

:hasDateInterval a owl:DatatypeProperty ;
	rdfs:domain :DateInformation ;
	rdfs:range xsd:string ;
	rdfs:comment "A single letter that records an interval assocated with the date: S=single, B=before and A=after." .
# 
# http://romanrepublic.ac.uk/rdf/ontology#hasDateSourceText

:hasDateSourceText a owl:DatatypeProperty ;
	rdfs:domain :AssertionWithDateRange ;
	rdfs:range xsd:string ;
	rdfs:comment "A field to contain a human-readable interpretation of the range of dates to which a status or post applied.  Whereas the associated year numeric fields :hasDateState and :hasDateEnd have perharps a rather \"cut and dried\" character to them (e.g. 52-50 BC), this interpretation string allows a more subtle statement about the date range to be made (\"ca. 51 BC\")." ;
	rdfs:seeAlso ":hasDateDisplayText (which was meant to provide a similar function to :hasDateSourceText but has been little used." .
# 
# http://romanrepublic.ac.uk/rdf/ontology#hasDateStart

:hasDateStart a owl:DatatypeProperty ;
	rdfs:domain :AssertionWithDateRange ;
	rdfs:range xsd:integer ;
	rdfs:comment "Provides the starting point (year) for the period of time that the assertion covers." .
# 
# http://romanrepublic.ac.uk/rdf/ontology#hasDescription

:hasDescription a owl:DatatypeProperty ;
	rdfs:domain :AuthorityWithDescription ;
	rdfs:range xsd:string ;
	rdfs:comment "provides the text for the description associated with the instance of the particular authority list." .
# 
# http://romanrepublic.ac.uk/rdf/ontology#hasDprrID

:hasDprrID a owl:DatatypeProperty ;
	rdfs:domain :Person ;
	rdfs:range xsd:string ;
	rdfs:comment "A short string made up of the first four letters of the person's Nomen and a four digit value of their key (ID). As the name suggest, could, at some point in the future, become a formal ID for the person in DPRR, rather than the numeric ID/key." .
# 
# http://romanrepublic.ac.uk/rdf/ontology#hasEraDisplayText

:hasEraDisplayText a owl:DatatypeProperty ;
	rdfs:domain :Person ;
	rdfs:range xsd:string ;
	rdfs:comment "A field to contain a comment about the range of dates when DPRR believed a person lived.  Rarely used." .
# 
# http://romanrepublic.ac.uk/rdf/ontology#hasEraFrom

:hasEraFrom a owl:DatatypeProperty ;
	rdfs:domain :Person ;
	rdfs:range xsd:integer ;
	rdfs:comment "A numeric field that provides the beginning date (year) for a date range in whid DPRR believes the person lived.  Often no birth or death date is available from the surviving record, so this is an estimate only." .
# 
# http://romanrepublic.ac.uk/rdf/ontology#hasEraTo

:hasEraTo a owl:DatatypeProperty ;
	rdfs:domain :Person ;
	rdfs:range xsd:integer ;
	rdfs:comment "A numeric field that provides the ending date (year) for a date range in whid DPRR believes the person lived.  Often no birth or death date is available from the surviving record, so this is an estimate only." .
# 
# http://romanrepublic.ac.uk/rdf/ontology#hasExtraInfo

:hasExtraInfo a owl:DatatypeProperty ;
	rdfs:domain :ThingWithExtraInfo ;
	rdfs:range xsd:string ;
	rdfs:comment "A place to record some prose text about many kinds of class instances in DPRR.  At the time of writing for this ontology, this property had not yet been used." .
# 
# http://romanrepublic.ac.uk/rdf/ontology#hasFiliation

:hasFiliation a owl:DatatypeProperty ;
	rdfs:domain :Person ;
	rdfs:range xsd:string ;
	rdfs:comment "A field for the filiation (a person's family member -- usually father) associated with a DPRR person and chosen to be recorded by the DPRR research team." .
# 
# http://romanrepublic.ac.uk/rdf/ontology#hasHighestOffice

:hasHighestOffice a owl:DatatypeProperty ;
	rdfs:domain :Person ;
	rdfs:range xsd:string ;
	rdfs:comment "A text property that describes what DPRR believes to be the highest office attained by the person." .
# 
# http://romanrepublic.ac.uk/rdf/ontology#hasID

:hasID a owl:DatatypeProperty ;
	rdfs:domain :ThingWithID ;
	rdfs:range xsd:integer ;
	rdfs:comment "The ID associated with an instance of class :ThingWithID.  All DPRR classes are subclasses of :ThingWithID, so all instances of all classes have a value for :hasID" .
# 
# http://romanrepublic.ac.uk/rdf/ontology#hasName

:hasName a owl:DatatypeProperty ;
	rdfs:domain :ThingWithName ;
	rdfs:range xsd:string ;
	rdfs:comment "The name of the thing." .
# 
# http://romanrepublic.ac.uk/rdf/ontology#hasNobilisNotes

:hasNobilisNotes a owl:DatatypeProperty ;
	rdfs:domain :Person ;
	rdfs:range xsd:string ;
	rdfs:comment "A note that records the reason why DPRR considers this person to have been thought of as a \"nobilis\".  Usually this takes the form of one or two brief primary source references." .
# 
# http://romanrepublic.ac.uk/rdf/ontology#hasNomen

:hasNomen a owl:DatatypeProperty ;
	rdfs:domain :Person ;
	rdfs:range xsd:string ;
	rdfs:comment "A text field containing the Nomen part of this DPRR person's name." .
# 
# http://romanrepublic.ac.uk/rdf/ontology#hasNoteText

:hasNoteText a owl:DatatypeProperty ;
	rdfs:domain :NoteContainer ;
	rdfs:range xsd:string ;
	rdfs:comment "the text of the note" .
# 
# http://romanrepublic.ac.uk/rdf/ontology#hasNotes

:hasNotes a owl:DatatypeProperty ;
	rdfs:domain :Assertion ;
	rdfs:range xsd:string ;
	rdfs:comment "Text of notes (primarily from secondary sources) that came with this particular information." .
# 
# http://romanrepublic.ac.uk/rdf/ontology#hasNovusNotes

:hasNovusNotes a owl:DatatypeProperty ;
	rdfs:domain :Person ;
	rdfs:range xsd:string ;
	rdfs:comment "A note that records the reason why DPRR considers this person to have been thought of as a \"novus\".  Usually this takes the form of one or two brief primary source references. Not much used." .
# 
# http://romanrepublic.ac.uk/rdf/ontology#hasOfficeXref

:hasOfficeXref a owl:DatatypeProperty ;
	rdfs:domain :PostAssertion ;
	rdfs:range xsd:string ;
	rdfs:comment "A text string associated with a Post Assertion which generally asserts the post in an abbreviated form: an abbrevation for the office (e.g. cos. for Consul) and the BCE year.  This text was taken primary from Broughton sources." .
# 
# http://romanrepublic.ac.uk/rdf/ontology#hasOrderNumber

:hasOrderNumber a owl:DatatypeProperty ;
	rdfs:domain :Relationship ;
	rdfs:range xsd:integer ;
	rdfs:comment "A number that provides a mechanism which provides a helpful ordering of a list of relationships from this table. If a list of relationships are generated, this number can be used to order them." .
# 
# http://romanrepublic.ac.uk/rdf/ontology#hasOrigin

:hasOrigin a owl:DatatypeProperty ;
	rdfs:domain :Person ;
	rdfs:range xsd:string ;
	rdfs:comment "A short bit of text that specifies what DPRR believes to be a plausible geographic origin for the person, as provided in the secondary and primary sources." .
# 
# http://romanrepublic.ac.uk/rdf/ontology#hasOriginalText

:hasOriginalText a owl:DatatypeProperty ;
	rdfs:domain :Assertion ;
	rdfs:range xsd:string ;
	rdfs:comment "Provides the original text, or an excerpt from it, as found in the source for the assertion." .
# 
# http://romanrepublic.ac.uk/rdf/ontology#hasOtherNames

:hasOtherNames a owl:DatatypeProperty ;
	rdfs:domain :Person ;
	rdfs:range xsd:string ;
	rdfs:comment "A text string in which DPRR records other names (beyond the usual 3 part nameing convention) that apply to the person." .
# 
# http://romanrepublic.ac.uk/rdf/ontology#hasPatricianNotes

:hasPatricianNotes a owl:DatatypeProperty ;
	rdfs:domain :Person ;
	rdfs:range xsd:string ;
	rdfs:comment "A note that records the reason why DPRR considers this person to have been thought of as a \"patrician\".  Usually this takes the form of one or two brief primary source references. This field was very rarely used by the DPRR team." .
# 
# http://romanrepublic.ac.uk/rdf/ontology#hasPersonName

:hasPersonName a owl:DatatypeProperty ;
	rdfs:subPropertyOf :hasName .
# 
# http://romanrepublic.ac.uk/rdf/ontology#hasPosition

:hasPosition a owl:DatatypeProperty ;
	rdfs:domain :PostAssertion ;
	rdfs:range xsd:integer ;
	rdfs:comment "A numeric value provided to assist web display mechanism to order posts in the most historically useful order." .
# 
# http://romanrepublic.ac.uk/rdf/ontology#hasProvinceOriginal

:hasProvinceOriginal a owl:DatatypeProperty ;
	rdfs:domain :PostAssertion ;
	rdfs:range xsd:string ;
	rdfs:comment "A text string taken from the secondary source that identifies the province associated with the post. A link to the structured version of the province (:Province) can be found through class :PostAssertionProvince." .
# 
# http://romanrepublic.ac.uk/rdf/ontology#hasProvinceOriginalExpanded

:hasProvinceOriginalExpanded a owl:DatatypeProperty ;
	rdfs:domain :PostAssertion ;
	rdfs:range xsd:string ;
	rdfs:comment "A text string providing an expanded form of a province name (created by DPRR) taken from the secondary source that identifies the province associated with the post. A link to the structured version of the province (:Province) can be found through class :PostAssertionProvince." .
# 
# http://romanrepublic.ac.uk/rdf/ontology#hasReNumber

:hasReNumber a owl:DatatypeProperty ;
	rdfs:domain :Person ;
	rdfs:range xsd:string ;
	rdfs:comment "The reference to the person in the Real-Encyclopädie der classischen Altertumswissenschaft (Pauly et al 1893-)." .
# 
# http://romanrepublic.ac.uk/rdf/ontology#hasReNumberOld

:hasReNumberOld a owl:DatatypeProperty ;
	rdfs:domain :Person ;
	rdfs:range xsd:string ;
	rdfs:comment "The reference used in the past (earlier schoalrship) to the person in the Real-Encyclopädie der classischen Altertumswissenschaft (Pauly et al 1893-). When provided, this has been supplanted by DPRR's more current view on which RE number is appropriate, as recorded in :hasReNumber." .
# 
# http://romanrepublic.ac.uk/rdf/ontology#hasRelationshipNumber

:hasRelationshipNumber a owl:DatatypeProperty ;
	rdfs:domain :RelationshipAssertion ;
	rdfs:range xsd:integer ;
	rdfs:comment "allows collection of relationahip assertions for a particular person to be sorted in the most temporarily appropriate order: sons usually after brothers, wives in the right order, etc etc." .
# 
# http://romanrepublic.ac.uk/rdf/ontology#hasSourceText

:hasSourceText a owl:DatatypeProperty ;
	rdfs:domain :DateInformation ;
	rdfs:range xsd:string .
# 
# http://romanrepublic.ac.uk/rdf/ontology#hasValue

:hasValue a owl:DatatypeProperty ;
	rdfs:domain :DateInformation ;
	rdfs:range xsd:integer ;
	rdfs:comment "The year associated with this life date." .
# 
# http://romanrepublic.ac.uk/rdf/ontology#isCognomenUncertain

:isCognomenUncertain a owl:DatatypeProperty ;
	rdfs:domain :Person ;
	rdfs:range xsd:boolean ;
	rdfs:comment "if true indicates that the DPRR team believe that the recorded Cognomen for this person is uncertain.  This property is only provided in the data if it is true." .
# 
# http://romanrepublic.ac.uk/rdf/ontology#isDateEndUncertain

:isDateEndUncertain a owl:DatatypeProperty ;
	rdfs:domain :Assertion ;
	rdfs:range xsd:boolean ;
	rdfs:comment "A boolean to indicate whether the end date in :hasDateEnd is uncertain.  Recorded only if \"true\"." .
# 
# http://romanrepublic.ac.uk/rdf/ontology#isDateStartUncertain

:isDateStartUncertain a owl:DatatypeProperty ;
	rdfs:domain :Assertion ;
	rdfs:range xsd:boolean ;
	rdfs:comment "A boolean to indicate whether the start date in :hasDateStart is uncertain.  Recorded only if \"true\"." .
# 
# http://romanrepublic.ac.uk/rdf/ontology#isFiliationUncertain

:isFiliationUncertain a owl:DatatypeProperty ;
	rdfs:domain :Person ;
	rdfs:range xsd:boolean ;
	rdfs:comment "if true indicates that the DPRR team believe that the recorded Filiation provided here for this person is uncertain.  This property is only provided in the data if it is true." .
# 
# http://romanrepublic.ac.uk/rdf/ontology#isNobilis

:isNobilis a owl:DatatypeProperty ;
	rdfs:domain :Person ;
	rdfs:range xsd:boolean ;
	rdfs:comment "is true if DPRR believes that the person was considered a \"nobilis\".  Only asserted if true." .
# 
# http://romanrepublic.ac.uk/rdf/ontology#isNobilisUncertain

:isNobilisUncertain a owl:DatatypeProperty ;
	rdfs:domain :Person ;
	rdfs:range xsd:boolean ;
	rdfs:comment "if true indicates that the DPRR team believe that the recorded \"nobilis\" provided here for this person is uncertain.  This property is only provided in the data if it is true." .
# 
# http://romanrepublic.ac.uk/rdf/ontology#isNomenUncertain

:isNomenUncertain a owl:DatatypeProperty ;
	rdfs:domain :Person ;
	rdfs:range xsd:boolean ;
	rdfs:comment "if true indicates that the DPRR team believe that the recorded Nomen provided here for this person is uncertain.  This property is only provided in the data if it is true." .
# 
# http://romanrepublic.ac.uk/rdf/ontology#isNovus

:isNovus a owl:DatatypeProperty ;
	rdfs:domain :Person ;
	rdfs:range xsd:boolean ;
	rdfs:comment "is true if DPRR believes that the person was considered a \"novus\".  Only asserted if true." .
# 
# http://romanrepublic.ac.uk/rdf/ontology#isNovusUncertain

:isNovusUncertain a owl:DatatypeProperty ;
	rdfs:domain :Person ;
	rdfs:range xsd:boolean ;
	rdfs:comment "if true indicates that the DPRR team believe that the assertion that this person was considered a Novus that is provided here for this person is uncertain.  This property is only provided in the data if it is true." .
# 
# http://romanrepublic.ac.uk/rdf/ontology#isOtherNamesUncertain

:isOtherNamesUncertain a owl:DatatypeProperty ;
	rdfs:domain :Person ;
	rdfs:range xsd:boolean ;
	rdfs:comment "if true indicates that the DPRR team believe that the \"other names\" provided here for this person is uncertain.  This property is only provided in the data if it is true." .
# 
# http://romanrepublic.ac.uk/rdf/ontology#isPatrician

:isPatrician a owl:DatatypeProperty ;
	rdfs:domain :Person ;
	rdfs:range xsd:boolean ;
	rdfs:comment "is true if DPRR believes that the person was considered a \"patrician\".  Only asserted if true." .
# 
# http://romanrepublic.ac.uk/rdf/ontology#isPatricianUncertain

:isPatricianUncertain a owl:DatatypeProperty ;
	rdfs:domain :Person ;
	rdfs:range xsd:boolean ;
	rdfs:comment "if true indicates that the DPRR team believe that the assertion that this person was a Patrician provided here is uncertain.  This property is only provided in the data if it is true." .
# 
# http://romanrepublic.ac.uk/rdf/ontology#isPraenomenUncertain

:isPraenomenUncertain a owl:DatatypeProperty ;
	rdfs:domain :Person ;
	rdfs:range xsd:boolean ;
	rdfs:comment "if true indicates that the DPRR team believe that the Praenomen provided here for this person is uncertain.  This property is only provided in the data if it is true." .
# 
# http://romanrepublic.ac.uk/rdf/ontology#isProvinceUncertain

:isProvinceUncertain a owl:DatatypeProperty ;
	rdfs:domain :NoteForProvince ;
	rdfs:range xsd:boolean ;
	rdfs:comment "When true, specifies that the connection to the given Province is uncertain.  Only appears if \"true\"." .
# 
# http://romanrepublic.ac.uk/rdf/ontology#isUncertain

:isUncertain a owl:DatatypeProperty ;
	rdfs:domain :Assertion ;
	rdfs:range xsd:boolean ;
	rdfs:comment "When true, specifies that the information in the Aseertion is uncertain.  Only appears if \"true\"." .
# 
# 
# 
# #################################################################
# #
# #    Classes
# #
# #################################################################
# 
# 
# http://romanrepublic.ac.uk/rdf/ontology#Assertion

:Assertion a owl:Class ;
	rdfs:subClassOf :ThingWithID ;
	rdfs:comment "In DPRR an :Assertion is a statement made about a DPRR person in a secondary source." .
# 
# http://romanrepublic.ac.uk/rdf/ontology#AssertionWithDateRange

:AssertionWithDateRange a owl:Class ;
	rdfs:subClassOf :Assertion ;
	rdfs:comment "some assertions come with a date period (year in which a post was held, for example).  This kind of :Assertion supports the recording of a date." .
# 
# http://romanrepublic.ac.uk/rdf/ontology#AuthorityList

:AuthorityList a owl:Class ;
	rdfs:subClassOf :ThingWithName ;
	rdfs:comment "represents a list of a particular kind of things that might be thought of as functioning like what in library science is called an Authority File.  Two examples: one Authority list in DPRR is the list of offices, another is the list of secondary sources." .
# 
# http://romanrepublic.ac.uk/rdf/ontology#AuthorityWithAbbreviation

:AuthorityWithAbbreviation a owl:Class ;
	rdfs:subClassOf :AuthorityList ;
	rdfs:comment "In DPRR several authority lists provide not only names for their instances, but also abbreviated forms of the name.  This is the place where the abbreviated form is recorded." .
# 
# http://romanrepublic.ac.uk/rdf/ontology#AuthorityWithDescription

:AuthorityWithDescription a owl:Class ;
	rdfs:subClassOf :AuthorityList ;
	rdfs:comment "In DPRR several authority lists provide not only names for their instances, but also brief descriptions of that the instance is.  This is the place where the description is recorded." .
# 
# http://romanrepublic.ac.uk/rdf/ontology#DateInformation

:DateInformation a owl:Class ;
	rdfs:subClassOf :Assertion ;
	rdfs:comment "An :Assertion for life date information for DPRR's historial persons." ;
	rdfs:label "Life Date Information" .
# 
# http://romanrepublic.ac.uk/rdf/ontology#DateType

:DateType a owl:Class ;
	rdfs:subClassOf :AuthorityWithDescription ;
	rdfs:comment "A classification scheme for kinds of life dates.  Examples, birth, death, exiled, etc." ;
	rdfs:label "Date Type" .
# 
# http://romanrepublic.ac.uk/rdf/ontology#HierarchicalAuthority

:HierarchicalAuthority a owl:Class ;
	rdfs:subClassOf :AuthorityList ;
	rdfs:comment "this authority list has an hierarichal structure between its members." .
# 
# http://romanrepublic.ac.uk/rdf/ontology#Note

:Note a owl:Class ;
	rdfs:subClassOf :NoteContainer ;
	rdfs:comment "A note is  a bit of text, often provided by the source to say something further about the information provided by it.  :Note is a subclass of :NoteContainer.  Whereas a note is purely and simply a note, its :NoteContainer superclass may also contain other information as well as the note." .
# 
# http://romanrepublic.ac.uk/rdf/ontology#NoteContainer

:NoteContainer a owl:Class ;
	rdfs:subClassOf :ThingWithID ;
	rdfs:comment "A note container is an object that contains a note:  a bit of text, often provided by the source to say something further about the information provided by it.  A note container object may also contain other information provided by the source, whereas its subclass :Note is purely a note with no other semantic significance." .
# 
# http://romanrepublic.ac.uk/rdf/ontology#NoteForProvince

:NoteForProvince a owl:Class ;
	rdfs:subClassOf :NoteContainer ;
	rdfs:comment "This is a note about an association to a Province made by an assertion." .
# 
# http://romanrepublic.ac.uk/rdf/ontology#NoteType

:NoteType a owl:Class ;
	rdfs:subClassOf :AuthorityWithDescription ;
	rdfs:comment "A scheme for classifying notes.  Draws almost exclusively on the classification of materials used by Broughton and Ruepke" ;
	rdfs:label "Note Type" .
# 
# http://romanrepublic.ac.uk/rdf/ontology#Office

:Office a owl:Class ;
	rdfs:subClassOf :AuthorityWithAbbreviation , :AuthorityWithDescription , :HierarchicalAuthority ;
	rdfs:comment "An office in the Roman state, such as consul or praetor." ;
	rdfs:label "Office" .
# 
# http://romanrepublic.ac.uk/rdf/ontology#Person

:Person a owl:Class ;
	rdfs:subClassOf :ThingWithExtraInfo , :ThingWithName ;
	rdfs:comment "A DPRR historical person." ;
	rdfs:label "Person" .
# 
# http://romanrepublic.ac.uk/rdf/ontology#PersonNote

:PersonNote a owl:Class ;
	rdfs:subClassOf :Note , :ThingWithExtraInfo ;
	rdfs:comment "A note attached to a DPRR person" ;
	rdfs:label "Person Note" .
# 
# http://romanrepublic.ac.uk/rdf/ontology#PostAssertion

:PostAssertion a owl:Class ;
	rdfs:subClassOf :AssertionWithDateRange ;
	rdfs:comment "provides an mechanism that a DPRR person held a particular office at a particular date or date range." ;
	rdfs:label "Post Assertion" .
# 
# http://romanrepublic.ac.uk/rdf/ontology#PostAssertionNote

:PostAssertionNote a owl:Class ;
	rdfs:subClassOf :Note , :ThingWithExtraInfo ;
	rdfs:comment "for notes associated with post assertions.  Broughton often provides text that supports his assertions, and many of the :PostAssertionNote items are from his book." ;
	rdfs:label "Post Assertion Note" .
# 
# http://romanrepublic.ac.uk/rdf/ontology#PostAssertionProvince

:PostAssertionProvince a owl:Class ;
	rdfs:subClassOf :NoteForProvince ;
	rdfs:comment "is used to link a :PostAssertion to an associated :Province." ;
	rdfs:label "Post Assertion Province" .
# 
# http://romanrepublic.ac.uk/rdf/ontology#Praenomen

:Praenomen a owl:Class ;
	rdfs:subClassOf :AuthorityWithAbbreviation ;
	rdfs:comment "A list of ancient Roman's first or personal name, for example *Marcus* Tullius Cicero.  The Romans seem to have used a relatively small numer of names as Praenomen." ;
	rdfs:label "Praenomen" .
# 
# http://romanrepublic.ac.uk/rdf/ontology#PrimarySource

:PrimarySource a owl:Class ;
	rdfs:subClassOf :Source ;
	rdfs:comment "An historical textual source" ;
	rdfs:label "Primary Source" .
# 
# http://romanrepublic.ac.uk/rdf/ontology#PrimarySourceReference

:PrimarySourceReference a owl:Class ;
	rdfs:subClassOf :NoteContainer ;
	rdfs:comment "A place to record primary source references.  The primary source data has not been worked on in DPRR.  It is a :NoteContainer because, as well as its primary founction, it also can carry a note." ;
	rdfs:label "Primary Source Reference" .
# 
# http://romanrepublic.ac.uk/rdf/ontology#Province

:Province a owl:Class ;
	rdfs:subClassOf :AuthorityWithDescription , :HierarchicalAuthority ;
	rdfs:comment "An area of jurisdition for an office (such as governor) in the Roman State. Most are geographic areas, but some represent domains of authority within the state, e.g. \"cum imperio consulari\"." ;
	rdfs:label "Province" .
# 
# http://romanrepublic.ac.uk/rdf/ontology#Relationship

:Relationship a owl:Class ;
	rdfs:subClassOf :AuthorityWithDescription ;
	rdfs:comment "This is the authority list for kinds of familial relationships that appear in DPRR." ;
	rdfs:label "Relationship Type" .
# 
# http://romanrepublic.ac.uk/rdf/ontology#RelationshipAssertion

:RelationshipAssertion a owl:Class ;
	rdfs:subClassOf :Assertion , :ThingWithExtraInfo ;
	rdfs:comment "Provides information about an assertion about a familial relationship between two people." ;
	rdfs:label "Relationship Assertion" .
# 
# http://romanrepublic.ac.uk/rdf/ontology#RelationshipAssertionReference

:RelationshipAssertionReference a owl:Class ;
	rdfs:subClassOf :Note , :ThingWithExtraInfo ;
	rdfs:comment "This class allows Relationahip Assertions to be connected to Secondary Sources from which the information in the assertion was drawn." ;
	rdfs:label "Relationship Assertion Reference" .
# 
# http://romanrepublic.ac.uk/rdf/ontology#RelationshipInverse

:RelationshipInverse a owl:Class ;
	rdfs:subClassOf :ThingWithID ;
	rdfs:comment "A class used to provide inverse relationships implied by primary ones.  For instance, A is father of B implies B is daughter of A is B is female, and B is son of A if B is male. In this class, for type or relationship in :forRelationship, when the sex of B is as provided in :forSex, then the appropriate inverse relationship is in :hasInverseRelationship" ;
	rdfs:label "Relationship Inverse" .
# 
# http://romanrepublic.ac.uk/rdf/ontology#SecondarySource

:SecondarySource a owl:Class ;
	rdfs:subClassOf :Source ;
	rdfs:comment "A modern source.  DPRR is primarily built by harvesting data from 19th, 20th and 21st century scholarship." ;
	rdfs:label "Secondary Source" .
# 
# http://romanrepublic.ac.uk/rdf/ontology#Sex

:Sex a owl:Class ;
	rdfs:subClassOf :AuthorityList ;
	rdfs:comment "The person's Sex: Male or Female." ;
	rdfs:label "Sex" .
# 
# http://romanrepublic.ac.uk/rdf/ontology#Source

:Source a owl:Class ;
	rdfs:subClassOf :AuthorityWithAbbreviation ;
	rdfs:comment "Represents a primary or secondary source that provided information for DPRR.  There are two subclasses :PrimarySource and :SecondarySource, but, because of time pressures, in fact only :SecondarySource has been populated by DPRR." .
# 
# http://romanrepublic.ac.uk/rdf/ontology#Status

:Status a owl:Class ;
	rdfs:subClassOf :AuthorityWithAbbreviation ;
	rdfs:comment "an authority list of status terms used for people in DPRR.  At present, only two are identified in this way, \"eques\" and \"senator\"" ;
	rdfs:label "Status" .
# 
# http://romanrepublic.ac.uk/rdf/ontology#StatusAssertion

:StatusAssertion a owl:Class ;
	rdfs:subClassOf :AssertionWithDateRange , :ThingWithExtraInfo ;
	rdfs:comment "provides a mechanism to assert that a person had a particular status at a particular time." ;
	rdfs:label "Status Assertion" .
# 
# http://romanrepublic.ac.uk/rdf/ontology#StatusAssertionNote

:StatusAssertionNote a owl:Class ;
	rdfs:subClassOf :Note , :ThingWithExtraInfo ;
	rdfs:comment "for notes associated with status assertions" ;
	rdfs:label "Status Assertion Note" .
# 
# http://romanrepublic.ac.uk/rdf/ontology#StatusAssertionProvince

:StatusAssertionProvince a owl:Class ;
	rdfs:subClassOf :NoteForProvince ;
	rdfs:comment "is used to link a :StatusAssertion to an associated :Province." ;
	rdfs:label "Status Assertion Province" .
# 
# http://romanrepublic.ac.uk/rdf/ontology#ThingWithExtraInfo

:ThingWithExtraInfo a owl:Class ;
	rdfs:subClassOf :ThingWithID .
# 
# http://romanrepublic.ac.uk/rdf/ontology#ThingWithID

:ThingWithID a owl:Class ;
	rdfs:comment "DPRR's source for RDF data is a relational database, and its mapping to RDF follows rather closely the DB's structure, in particular DPRR's tables to owl:Classes.  Thus, since all of DPRR's tables have ID keys, all DPRR[s classes have ID, and, hence, all DPRR classes are subclasses of :ThingWithID" .
# 
# http://romanrepublic.ac.uk/rdf/ontology#ThingWithName

:ThingWithName a owl:Class ;
	rdfs:subClassOf :ThingWithID ;
	rdfs:comment "An entity in DPRR that has a name.  Many DPRR classes represent things that have names, and are, thus, subclasses of this class." ;
	rdfs:label "Thing with Name" .
# 
# http://romanrepublic.ac.uk/rdf/ontology#Tribe

:Tribe a owl:Class ;
	rdfs:subClassOf :AuthorityWithAbbreviation , :ThingWithExtraInfo ;
	rdfs:comment "The tribes into which the ancient Roman's grouped themselves." ;
	rdfs:label "Tribe" .
# 
# http://romanrepublic.ac.uk/rdf/ontology#TribeAssertion

:TribeAssertion a owl:Class ;
	rdfs:subClassOf :Assertion ;
	rdfs:comment "An assertion that a DPRR person belonged to a particular tribe." ;
	rdfs:label "Tribe Assertion" .
# 
# 
# 
# #################################################################
# #
# #    Annotations
# #
# #################################################################
# 
# 

:hasPersonName rdfs:comment "The DPRR name-identifier assigned to a DPRR historical person. E.g. \"L. Iunius (46a, Supb. 5.356ff.) M. f. Brutus\" (for Person/1)" .
# 
# Generated by the OWL API (version 4.2.6.20160910-2108) https://github.com/owlcs/owlapi
